first comments for automatons

src/automatons/dAutomaton.thy
@@ -5,48 +5,73 @@ begin
 
 
 (*causes problems in sb.thy*)
-lemma prod_contI[cont2cont]: "(\<And>s. cont(\<lambda>f. g (f,s))) \<Longrightarrow>(\<And>f. cont (\<lambda>s. g (f,s))) \<Longrightarrow> cont g"
+lemma prod_contI[cont2cont]: "(\<And>s. cont(\<lambda>f. g (f,s))) 
+\<Longrightarrow>(\<And>f. cont (\<lambda>s. g (f,s))) \<Longrightarrow> cont g"
   by (simp add: prod_contI)
 (*>*)
 
-section \<open>Deterministic Automaton\<close>
+section\<open>Automatons \<close>
+
+text\<open>The behaviour of a component can be modeled by a I/O automaton.
+This section defines deterministic and non-deterministic automaton 
+types, defines their semantic mapping to \Gls{spf} and \Gls{SPS}.
+Furthermore, we take a closer look at causal automatons and use
+their properties to introduce a local that is capable of
+constructing automaton and is also providing lemmas to ease the 
+verification process for the input-output behavior.\<close>
+
+
+subsection \<open>Deterministic Automaton\<close>
 default_sort %invisible "chan"
 
-text\<open> \<close>
+text\<open>A deterministic I/O Automaton consists of states, a transition
+function, a initial state and a initial output. The transition
+function for deterministic automaton maps from a state with a
+@{type sbElem} to another state and a output \gls{sb}. Now we define
+deterministic automaton as a tuple.\<close>
 
-subsection \<open>Deterministic Automaton definition \<close>
-record ('state::type, 'in, 'out::chan) dAutomaton  =
+record ('state::type, 'in, 'out) dAutomaton  =
   daTransition :: "('state \<Rightarrow> 'in\<^sup>\<surd> \<Rightarrow> ('state \<times> 'out\<^sup>\<Omega>))"
   daInitState :: "'state"
   daInitOut:: "'out\<^sup>\<Omega>"
 
-subsubsection \<open>Deterministic Automaton general functions\<close>
+text\<open>The type parameter of @{type dAutomaton} show the state set and
+the input and output domain. We then introduce two definition to 
+obtain the next state or the next output of the transition function.
+\<close>
 
-definition daNextState:: "('s::type,'in::{chan, finite} , _) dAutomaton \<Rightarrow> 's \<Rightarrow>  'in\<^sup>\<surd> \<Rightarrow> 's" where
+definition daNextState:: 
+"('s::type,'in , _) dAutomaton \<Rightarrow> 's \<Rightarrow>  'in\<^sup>\<surd> \<Rightarrow> 's"where 
 "daNextState aut s m = fst ((daTransition aut) s m)"
 
-definition daNextOut:: "('s::type, 'in::{chan, finite},'out::chan) dAutomaton \<Rightarrow> 's \<Rightarrow>  'in\<^sup>\<surd> \<Rightarrow> 'out\<^sup>\<Omega>" where
+definition daNextOut::
+"('s::type, 'in,'out) dAutomaton \<Rightarrow> 's \<Rightarrow>  'in\<^sup>\<surd> \<Rightarrow> 'out\<^sup>\<Omega>" where
 "daNextOut aut s m = snd ((daTransition aut) s m)"
-
-subsection \<open>Semantic for deterministic Automaton \<close>
 
 subsubsection \<open>Semantic\<close>
 
-definition daStateSem :: "('s::type, 'I::{finite,chan},'O) dAutomaton \<Rightarrow> ('s \<Rightarrow> ('I\<^sup>\<Omega> \<rightarrow> 'O\<^sup>\<Omega>))" where
-"daStateSem da = fix\<cdot>(\<Lambda> h. (\<lambda> state. sb_split\<cdot>
-                        (\<lambda>sbe. \<Lambda> sb.
-                          let (nextState, output) = daTransition da state sbe in
-                            output \<bullet>\<^sup>\<Omega> h nextState\<cdot>sb)
-                      ))"
+definition daStateSem::"('s::type, 'I::{finite,chan},'O) dAutomaton 
+\<Rightarrow> ('s \<Rightarrow> ('I\<^sup>\<Omega> \<rightarrow> 'O\<^sup>\<Omega>))" where
+"daStateSem da =
+ fix\<cdot>(\<Lambda> h. (\<lambda> state. sb_split\<cdot>
+        (\<lambda>sbe. \<Lambda> sb.
+           let (nextState, output) = daTransition da state sbe in
+          output \<bullet>\<^sup>\<Omega> h nextState\<cdot>sb)))"
 
-definition daSem :: "('s::type, 'I::{finite,chan},'O) dAutomaton \<Rightarrow> ('I\<^sup>\<Omega> \<rightarrow> 'O\<^sup>\<Omega>)" where
-"daSem da = (\<Lambda> sb. (daInitOut da)\<bullet>\<^sup>\<Omega>((daStateSem da (daInitState da))\<cdot>sb))"
+definition daSem::"('s::type, 'I::{finite,chan},'O) dAutomaton 
+\<Rightarrow> ('I\<^sup>\<Omega> \<rightarrow> 'O\<^sup>\<Omega>)" where
+"daSem da \<equiv> \<Lambda> sb. daInitOut da \<bullet>\<^sup>\<Omega> daStateSem da(daInitState da)\<cdot>sb"
 
-subsubsection \<open>Statesemantic lemmas\<close>
 
-theorem dastatesem_unfolding: "(daStateSem automat s) = sb_split\<cdot>(\<lambda>sbe. \<Lambda> sb .
-                                                  let (nextState, output) = daTransition automat s sbe in
-                            output \<bullet>\<^sup>\<Omega> ((daStateSem automat) nextState\<cdot>sb))"
+paragraph\<open>Semantic Properties\<close>
+
+text\<open>\\\\\<close>
+text\<open>paragraph test \<close>
+
+theorem dastatesem_unfolding: "(daStateSem automat s) = 
+sb_split\<cdot>(\<lambda>sbe. \<Lambda> sb .
+           let (nextState, output) = daTransition automat s sbe in
+           output \<bullet>\<^sup>\<Omega> ((daStateSem automat) nextState\<cdot>sb))"
   unfolding daStateSem_def
   apply(subst fix_eq)
   apply(subst beta_cfun)
@@ -59,7 +84,8 @@ theorem dastatesem_bottom:
   shows "(daStateSem automat s)\<cdot>sb = \<bottom>"
   apply (subst dastatesem_unfolding)
   apply (simp add: sb_split_insert)
-  by (metis (no_types, lifting) assms fup1 sbHdElem_h_cont.rep_eq sbHdElem_h_def)
+  by (metis (no_types, lifting) assms fup1 sbHdElem_h_cont.rep_eq 
+      sbHdElem_h_def)
 
 lemma dastatesem_strict:
   assumes "\<not> chDomEmpty TYPE('b::{finite, chan})"
@@ -68,10 +94,12 @@ lemma dastatesem_strict:
 
 lemma dastatesem_step: 
   assumes "sbHdElemWell sb"
-  shows "(daStateSem da s)\<cdot>sb = snd (daTransition da s (sbHdElem sb)) \<bullet>\<^sup>\<Omega> daStateSem da (fst (daTransition da s (sbHdElem sb)))\<cdot>(sbRt\<cdot>sb)"
+  shows "(daStateSem da s)\<cdot>sb = snd (daTransition da s (sbHdElem sb)) 
+  \<bullet>\<^sup>\<Omega> daStateSem da (fst (daTransition da s (sbHdElem sb)))\<cdot>(sbRt\<cdot>sb)"
   apply (subst dastatesem_unfolding)
   apply (simp add: sb_split_insert Let_def case_prod_unfold)
-  apply (cases "sbHdElem_h_cont\<cdot>sb", simp_all add: sbHdElem_h_cont.rep_eq sbHdElem_def)
+  apply (cases "sbHdElem_h_cont\<cdot>sb")
+  apply (simp_all add: sbHdElem_h_cont.rep_eq sbHdElem_def)
   apply (simp_all split: u.split)
   apply (metis assms inst_up_pcpo sbHdElem_h_def u.simps(3))
   by (simp add: up_def)
@@ -79,29 +107,34 @@ lemma dastatesem_step:
 lemma dastatesem_final:
   assumes "sbHdElemWell sb"
   shows "(daStateSem automat s)\<cdot>sb =
-  (daNextOut automat s (sbHdElem sb)) \<bullet>\<^sup>\<Omega> (((daStateSem automat (daNextState automat s (sbHdElem sb))))\<cdot>(sbRt\<cdot>sb))"
+  daNextOut automat s (sbHdElem sb) \<bullet>\<^sup>\<Omega> 
+  daStateSem automat (daNextState automat s (sbHdElem sb))\<cdot>(sbRt\<cdot>sb)"
   by (metis assms daNextOut_def daNextState_def dastatesem_step)
 
 lemma dastatesem_final_h2:
   shows "(daStateSem automat s)\<cdot>(sbECons sbe\<cdot>sb) =
-  (daNextOut automat s sbe) \<bullet>\<^sup>\<Omega> ((daStateSem automat (daNextState automat s sbe))\<cdot>sb)"
+  (daNextOut automat s sbe) \<bullet>\<^sup>\<Omega> 
+  ((daStateSem automat (daNextState automat s sbe))\<cdot>sb)"
   apply (cases "chDomEmpty(TYPE('b))")
   apply (subst sbtypeepmpty_sbenone[of sbe],simp)+
   apply (subst sbtypeepmpty_sbbot[of sb],simp)+
   apply (subst dastatesem_unfolding, simp add: sb_split_insert)
   apply (subst case_prod_unfold)
-  apply (subgoal_tac "sbHdElem_h_cont\<cdot>\<bottom> = up\<cdot>(Abs_sbElem(None)::'b\<^sup>\<surd>)")
+  apply (subgoal_tac "sbHdElem_h_cont\<cdot>\<bottom>=up\<cdot>(Abs_sbElem(None)::'b\<^sup>\<surd>)")
   apply (simp add: daNextOut_def daNextState_def)
-  apply (simp add: sbHdElem_h_cont.rep_eq sbHdElem_h_def chDom_def up_def)
+  apply (simp add: sbHdElem_h_cont.rep_eq sbHdElem_h_def chDom_def 
+          up_def)
   apply (subst dastatesem_step)
   apply (simp add: sbECons_def sbHdElemWell_def)
   using sbgetch_sbe2sb_nempty strictI apply fastforce
-  by (simp only: daNextOut_def daNextState_def sbhdelem_sbecons sbrt_sbecons)
+  by (simp only: daNextOut_def daNextState_def sbhdelem_sbecons 
+      sbrt_sbecons)
 
 theorem dastatesem_stepI:
   assumes "(daNextOut da s sbe) = out"
-      and "(daNextState da s sbe) = nextState"
-  shows "(daStateSem da s)\<cdot>(sbECons sbe\<cdot>sb) = out  \<bullet>\<^sup>\<Omega> ((daStateSem da nextState)\<cdot>sb)"
+  and "(daNextState da s sbe) = nextState"
+  shows "daStateSem da s\<cdot>(sbe \<bullet>\<^sup>\<surd> sb) = 
+         out  \<bullet>\<^sup>\<Omega> daStateSem da nextState\<cdot>sb"
   by (simp add: assms dastatesem_final_h2)
 
 theorem dastatesem_inempty_len:
@@ -111,41 +144,57 @@ theorem dastatesem_inempty_len:
   shows "\<forall>s. sbLen (daStateSem automat s\<cdot>\<bottom>) = \<infinity>"
 proof(rule contrapos_pp,simp+)
   assume a1: "\<exists>s::'state. sbLen (daStateSem automat s\<cdot>\<bottom>) \<noteq> \<infinity>"
-  obtain len_set where len_set_def: "len_set = { sbLen (daStateSem automat s\<cdot>\<bottom>) | s. True }"
+  obtain len_set where len_set_def: 
+        "len_set = {sbLen (daStateSem automat s\<cdot>\<bottom>) | s. True }"
     by simp
   hence len_set_least: "\<exists>n \<in> len_set. \<forall>i \<in> len_set. n \<le> i"
-    by (metis (mono_tags, lifting) exists_least_iff le_less_linear len_set_def mem_Collect_eq)
-  then obtain state where state_def: "sbLen (daStateSem automat state\<cdot>\<bottom>) \<in> len_set" and "\<forall>n \<in> len_set. sbLen (daStateSem automat state\<cdot>\<bottom>) \<le> n"
+    by (metis (mono_tags, lifting) exists_least_iff le_less_linear 
+        len_set_def mem_Collect_eq)
+  then obtain state where state_def: "sbLen 
+    (daStateSem automat state\<cdot>\<bottom>) \<in> len_set" 
+    and "\<forall>n \<in> len_set. sbLen (daStateSem automat state\<cdot>\<bottom>) \<le> n"
     using len_set_def by blast
-  hence state_least: "\<forall>s. sbLen (daStateSem automat state\<cdot>\<bottom>) \<le> sbLen (daStateSem automat s\<cdot>\<bottom>)"
+  hence state_least: "\<forall>s. sbLen (daStateSem automat state\<cdot>\<bottom>) \<le> 
+                          sbLen (daStateSem automat s\<cdot>\<bottom>)"
     using len_set_def len_set_least by blast
-  then obtain k where k_def: "Fin k = sbLen (daStateSem automat state\<cdot>\<bottom>)"
+  then obtain k where k_def: "Fin k = 
+                              sbLen (daStateSem automat state\<cdot>\<bottom>)"
     by (metis SBv3.lnat.exhaust a1 inf_less_eq)
-  hence "Fin k < sbLen (daNextOut automat state (Abs_sbElem None)) + sbLen (daStateSem automat (daNextState automat state (Abs_sbElem None))\<cdot> \<bottom>)"
-    by (metis state_least add.commute assms(1) le2lnle leI lessequal_addition lnat_plus_suc notinfI3)
+  hence "Fin k < sbLen (daNextOut automat state (Abs_sbElem None)) + 
+         sbLen (daStateSem automat 
+         (daNextState automat state (Abs_sbElem None))\<cdot> \<bottom>)"
+    by (metis state_least add.commute assms(1) le2lnle leI 
+        lessequal_addition lnat_plus_suc notinfI3)
   thus "False"
-    by (metis assms(2) dastatesem_final_h2 k_def leD sblen_sbconc sbtypeempty_sbecons_bot)
+    by (metis assms(2) dastatesem_final_h2 k_def leD sblen_sbconc 
+        sbtypeempty_sbecons_bot)
 qed
 
 lemma dastatesem_weak_fin:
   assumes "sbLen sb = Fin n"
     and "\<And>state sbe. 1 \<le> sbLen (daNextOut automat state sbe)"
   shows "sbLen sb \<le> sbLen (daStateSem automat s\<cdot>sb)"
-  apply (induction sb arbitrary: s rule: sb_finind, simp_all add: assms)
-  apply(cases "chDomEmpty TYPE('a)")
+  apply (induction sb arbitrary: s rule: sb_finind)
+  apply (simp_all add: assms)
+  apply (cases "chDomEmpty TYPE('a)")
   using assms(1) apply auto[1]
   using sbleast2sblenempty apply fastforce
-  by (metis (no_types, lifting) dual_order.trans sbECons_def sbecons_len assms(2) dastatesem_final_h2 lessequal_addition lnat_plus_commu lnat_plus_suc sbECons_def sblen_sbconc)
+  by (metis (no_types, lifting) dual_order.trans sbECons_def 
+      sbecons_len assms(2) dastatesem_final_h2 lessequal_addition 
+      lnat_plus_commu lnat_plus_suc sbECons_def sblen_sbconc)
 
 theorem dastatesem_weak:
-  assumes "\<And>state sbe. 1 \<le> sbLen (daNextOut (automat::('state, 'in::{chan, finite}, 'out) dAutomaton) state sbe)"
+  fixes automat::"('state, 'in::{chan, finite}, 'out) dAutomaton"
+  assumes "\<And>state sbe. 1 \<le> sbLen (daNextOut automat state sbe)"
   shows     "weak_well (daStateSem automat s)"
   apply (cases "chDomEmpty TYPE('in)")
-  apply (metis (full_types) assms dastatesem_inempty_len fold_inf less_lnsuc sblen_empty sbtypeepmpty_sbbot weak_well_def)
+  apply (metis (full_types) assms dastatesem_inempty_len fold_inf 
+        less_lnsuc sblen_empty sbtypeepmpty_sbbot weak_well_def)
   by (metis assms spf_weakI2 dastatesem_weak_fin lnat_well_h2)
 
 theorem dastatesem_least:
-  assumes"(\<lambda>state. sb_split\<cdot>(\<lambda>sbe. \<Lambda> sb. snd (daTransition X state sbe) \<bullet>\<^sup>\<Omega>  
+  assumes"(\<lambda>state. sb_split\<cdot>
+          (\<lambda>sbe. \<Lambda> sb. snd (daTransition X state sbe) \<bullet>\<^sup>\<Omega>  
           Z (fst (daTransition X state sbe))\<cdot>sb)) \<sqsubseteq> Z"
   shows"daStateSem X \<sqsubseteq> Z"
   apply (simp add: daStateSem_def)
@@ -154,10 +203,9 @@ theorem dastatesem_least:
   apply (intro cont2cont; simp)
   by (simp add: assms case_prod_unfold)
   
-subsubsection \<open>Semantic lemmas\<close>
-
 theorem dasem_insert:
-  "daSem automat\<cdot>sb = (daInitOut automat) \<bullet>\<^sup>\<Omega> ((daStateSem automat (daInitState automat))\<cdot>sb)"
+  "daSem automat\<cdot>sb = daInitOut automat \<bullet>\<^sup>\<Omega> 
+                     daStateSem automat (daInitState automat)\<cdot>sb"
   by (simp add: daSem_def)
 
 theorem dasem_bottom:
@@ -173,17 +221,26 @@ theorem dasem_strong:
   apply (simp add: daSem_def)
 proof
   fix sb
-  have h1: "sbLen sb <\<^sup>l lnsuc\<cdot>(sbLen (daStateSem automat (daInitState automat)\<cdot>sb))"
+  have h1: "sbLen sb <\<^sup>l lnsuc\<cdot>(sbLen 
+                      (daStateSem automat (daInitState automat)\<cdot>sb))"
     using assms(1) sblen_mono
     by (simp add: weak_well_def)
-  have h4: "lnsuc\<cdot>(sbLen (daStateSem automat (daInitState automat)\<cdot>sb)) \<le> sbLen (daInitOut automat) + sbLen (daStateSem automat (daInitState automat)\<cdot>sb)"
-    using assms(2) lessequal_addition lnat_plus_commu lnat_plus_suc by fastforce 
-  have h2: "sbLen (daInitOut automat) + sbLen (daStateSem automat (daInitState automat)\<cdot>sb) \<le> sbLen (daInitOut automat \<bullet>\<^sup>\<Omega>  daStateSem automat (daInitState automat)\<cdot>sb)"
+  have h4: "lnsuc\<cdot>(sbLen(daStateSem automat(daInitState automat)\<cdot>sb))
+             \<le> sbLen (daInitOut automat) + 
+               sbLen (daStateSem automat (daInitState automat)\<cdot>sb)"
+    by (metis add.commute assms(2) lessequal_addition lnat_plus_suc 
+        order_refl)
+  have h2: "sbLen (daInitOut automat) + sbLen (daStateSem automat 
+       (daInitState automat)\<cdot>sb) \<le> sbLen (daInitOut automat \<bullet>\<^sup>\<Omega>  
+        daStateSem automat (daInitState automat)\<cdot>sb)"
     using sblen_sbconc by auto
-  have h3: "sbLen sb <\<^sup>l sbLen (daInitOut automat \<bullet>\<^sup>\<Omega> daStateSem automat (daInitState automat)\<cdot>sb)"
+  have h3: "sbLen sb <\<^sup>l sbLen (daInitOut automat \<bullet>\<^sup>\<Omega> 
+            daStateSem automat (daInitState automat)\<cdot>sb)"
     using h1 h2 h4 dual_order.trans by blast
-  then show "\<And>sb. sbLen sb <\<^sup>l sbLen (daInitOut automat \<bullet>\<^sup>\<Omega>  daStateSem automat (daInitState automat)\<cdot>sb)"
-    by (metis assms(1) assms(2) dual_order.trans lessequal_addition lnat_plus_commu lnat_plus_suc sblen_sbconc weak_well_def)
+  then show "\<And>sb. sbLen sb <\<^sup>l sbLen (daInitOut automat \<bullet>\<^sup>\<Omega>  
+                  daStateSem automat (daInitState automat)\<cdot>sb)"
+    by (metis assms(1) assms(2) dual_order.trans lessequal_addition 
+        lnat_plus_commu lnat_plus_suc sblen_sbconc weak_well_def)
 qed
 
 (*<*)
